clean up

Stlc/Classes.v
@@ -22,94 +22,145 @@ Class Subst (e : nat -> Set) (u : nat -> Set) `{Syntax e} `{Syntax u} := {
 (** * Theory *)
 (***********************************************************************)
 
-(* These are the general form of the lemmas in the Lemmas.v file; and 
-   perhaps automatically proven by a future version of LNgen. *)
+(* These are the general form of the lemmas in the Lemmas.v file. *)
    
 
 Class SyntaxTheory (exp : nat -> Set) `{H: Syntax exp} := {
 
-   size_weaken : forall n (t : exp n), size (weaken t) = size t;
+    size_weaken : forall n (t : exp n), size (weaken t) = size t;
 
-   fv_weaken : forall n1 (e1 : exp n1), fv (weaken e1) = fv e1;
-
-   size_min : forall n (e : exp n), 1 <= size e;
-
-   size_close : forall n (e1 : exp n) x1, 
+    fv_weaken : forall n1 (e1 : exp n1), fv (weaken e1) = fv e1;
+    
+    size_min : forall n (e : exp n), 1 <= size e;
+    
+    size_close : forall n (e1 : exp n) x1, 
       size (close x1 e1) = size e1;
-
-   close_inj : (forall k (e1 : exp k) e2 x1,
+    
+    close_inj : forall k (e1 : exp k) e2 x1,
       close x1 e1 = close x1 e2 ->
-      e1 = e2);
+      e1 = e2;
 
-  close_weaken : (forall n1 (e1 : exp n1) x1,
-                      x1 `notin` fv e1 ->
-                      close x1 e1 = weaken e1);
-
-(*
-  fv_close := fv_exp_close_exp_wrt_exp;
-  fv_subst_fresh := fv_exp_subst_exp_wrt_exp_fresh;
-  fv_subst_lower := fv_exp_subst_exp_wrt_exp_lower;
-  fv_subst_notin := fv_exp_subst_exp_wrt_exp_notin;
-  fv_subst_upper := fv_exp_subst_exp_wrt_exp_upper; *)
-
-
-   (* TODO: add more *)
-   }.
-
-(* TODO: rewriting/hint database for the above lemmas. *)
-
-
-Class SubstTheory (exp : nat -> Set) (u : nat -> Set) (uvar : forall {n}, atom -> u n) `{H: Subst exp u} := {
-
-   size_open : (forall k (e1 : exp (S k)) (e2 :u k),
-      size e1 <= size (open e2 e1));
-
-   size_open_var : (forall k (e : exp (S k)) x,
-      size (open (uvar x) e) = size e);
-
-   close_open : (forall n1 (e1 : exp (S n1)) x1 ,
+   close_weaken : forall n1 (e1 : exp n1) x1,
       x1 `notin` fv e1 ->
-      close x1 (open (uvar x1) e1) = e1);
+      close x1 e1 = weaken e1;
 
-   open_close : (forall n1 (e1 : exp n1) x1,
-      open (uvar x1) (close x1 e1) = e1);
+    fv_close : forall n1 (e1 : exp n1) x1,
+      fv (close x1 e1) [=] remove x1 (fv e1);
+}.
 
-   open_inj : (forall n1 (e2 e1:exp (S n1)) x1,
+
+Class SubstTheory (exp : nat -> Set) (u : nat -> Set) 
+      `{H: Subst exp u} := {
+    
+    size_open : forall k (e1 : exp (S k)) (e2 :u k),
+      size e1 <= size (open e2 e1);
+        
+    open_weaken : forall n1 (e2 : exp n1) e1,
+      open e1 (weaken e2) = e2;
+
+    fv_open_lower : forall n1 (e1 : exp (S n1)) e2,
+      fv e1 [<=] fv (open e2 e1);
+
+    fv_open_upper : forall n1 (e1 : exp (S n1)) e2,
+      fv (open e2 e1) [<=] fv e2 `union` fv e1;
+
+
+    fv_subst_fresh : forall n1 (e1 : exp n1) e2 x1,
+      x1 `notin` fv e1 ->
+      fv (subst e2 x1 e1) [=] fv e1;
+
+    fv_subst_lower : forall n1 (e1 : exp n1) e2 x1,
+      remove x1 (fv e1) [<=] fv (subst e2 x1 e1);
+
+    fv_subst_notin : forall n1 (e1 : exp n1) e2 x1 x2,
+      x2 `notin` fv e1 ->
+      x2 `notin` fv e2 ->
+      x2 `notin` fv (subst e2 x1 e1);
+
+    fv_subst_upper : forall n1 (e1 : exp n1) e2 x1,
+      fv (subst e2 x1 e1) [<=] fv e2 `union` remove x1 (fv e1);  
+
+    subst_close : forall n1 (e2 : exp n1) e1 x1 x2,
+      x1 <> x2 ->
+      x2 `notin` fv e1 ->
+      subst (weaken e1) x1 (close x2 e2) =
+        close x2 (subst e1 x1 e2);
+
+    subst_fresh_eq : forall n1 (e2 : exp n1) e1 x1,
+      x1 `notin` fv e2 ->
+      subst e1 x1 e2 = e2;
+    
+    subst_fresh_same : forall n1 (e2 : exp n1) e1 x1,
+      x1 `notin` fv e1 ->
+      x1 `notin` fv (subst e1 x1 e2);
+
+
+    subst_weaken : forall n u1 x1 (e1:exp n),
+      weaken (subst u1 x1 e1) = 
+        subst (weaken u1) x1 (weaken e1);  
+
+   subst_spec : forall n (e1 : exp n) e2 x1,
+      subst e2 x1 e1 = open e2 (close x1 e1);
+                                                          
+  }.
+
+Class SubstVarTheory (exp : nat -> Set) (u : nat -> Set) 
+      (uvar : forall {n}, atom -> u n) `{H: Subst exp u} := {
+
+    size_open_var : forall k (e : exp (S k)) x,
+      size (open (uvar x) e) = size e;
+
+    close_open : forall n1 (e1 : exp (S n1)) x1 ,
+      x1 `notin` fv e1 ->
+      close x1 (open (uvar x1) e1) = e1;
+
+    open_close : forall n1 (e1 : exp n1) x1,
+      open (uvar x1) (close x1 e1) = e1;
+    
+    open_inj : forall n1 (e2 e1:exp (S n1)) x1,
       x1 `notin` fv e2 ->
       x1 `notin` fv e1 ->
       open (uvar x1) e2 = open (uvar x1) e1 ->
-      e2 = e1);
-
-   open_weaken : (forall n1 (e2 : exp n1) e1,
-                     open e1 (weaken e2) = e2);
-
-   subst_intro  : forall n (e1 : exp (S n)) (x1:atom) (e2 : u n),
-      x1 `notin` fv e1 ->
-      open e2 e1 = subst e2 x1 (open (uvar x1) e1) ;
+      e2 = e1;
 
    subst_open_var : forall n1 (e2 : exp (S n1)) e1 x1 x2,
         x1 <> x2 ->
         open (uvar x2) (subst (weaken e1) x1 e2) = 
-          subst e1 x1 (open (uvar x2) e2)
-  (* 
-  fv_open_lower := fv_exp_open_exp_wrt_exp_lower;
-  fv_open_upper := fv_exp_open_exp_wrt_exp_upper;
-  *)
+          subst e1 x1 (open (uvar x2) e2);
+   subst_close_open : forall n1 (e2 : exp (S n1)) e1 x1 x2,
+      x2 `notin` fv e2 ->
+      x2 `notin` fv e1 ->
+      x2 <> x1 ->
+      subst (weaken e1) x1 e2 = 
+      close x2 
+       (subst e1 x1 (open (uvar x2) e2)); 
 
+   subst_intro  : forall n (e1 : exp (S n)) (x1:atom) (e2 : u n),
+      x1 `notin` fv e1 ->
+      open e2 e1 = subst e2 x1 (open (uvar x1) e1) ;
+}.
+
+Class SubstSubstTheory (exp : nat -> Set) (u : nat -> Set) 
+      `{H: Subst exp u}`{HU: Subst u u} := {
+
+    subst_open : forall n1 (e1 : u n1) e2 (e3 : exp (S n1)) x1,
+      subst e1 x1 (open e2 e3) =
+        open (subst e1 x1 e2) (subst (weaken e1) x1 e3);  
+    
+    subst_subst : forall n (e1 : exp n) e2 e3 x2 x1,
+      x2 `notin` fv e2 ->
+      x2 <> x1 ->
+      subst e2 x1 (subst e3 x2 e1) = 
+        subst (subst e2 x1 e3) x2 (subst e2 x1 e1); 
   }.
 
+
+
+(***********************************************************************)
+(** * Rewriting / tactics *)
+(***********************************************************************)
+
 Create HintDb syntax.
-
-(*
-Hint Rewrite (fun {e} {u} {v} `{K:SubstTheory e u v} => @close_open e u v _ _) 
-  using solve [auto; try typeclasses eauto] : syntax.
-
-Hint Rewrite (fun {e} {u} {v} `{K:SubstTheory e u v} => @open_close e u v _ _) 
-  using solve [auto; try typeclasses eauto] : syntax.
-
-Hint Rewrite (fun {e} {u} {v} `{K:SubstTheory e u v} => @subst_open_var e u v _ _) 
-  using solve [auto; try typeclasses eauto] : syntax.
-*)
 
 Hint Rewrite  @close_open
   using solve [auto; try typeclasses eauto] : syntax.
@@ -119,11 +170,6 @@ Hint Rewrite @open_close
 
 Hint Rewrite @subst_open_var
   using solve [auto; try typeclasses eauto] : syntax.
-
-
-(***********************************************************************)
-(** * Rewriting / tactics *)
-(***********************************************************************)
 
 
 Create HintDb fv.
