Stlc/Fin.v
@@ -2,18 +2,26 @@
 (** * Definition of Finite numbers *)
 (***********************************************************************)
 
-(* Bound variables are represented using the 'fin' datatype shown below. 
-The key idea is the index of this type says how many elements it has. For 
-example, the type [fin 0] is an empty type, the type [fin 1] only has a 
-single value [fO], the type [fin 2] has two values ([fO] and [fS fO]). *)
+(* Bound variables are represented using the 'fin' datatype shown below.
+
+   Elements of fin n can be seen as natural numbers in the set {m | m < n}.
+
+   The key idea is the index of this type says how many elements the type
+   has. For example, the type [fin 0] is an empty type, the type [fin 1] only
+   has a single value [fO], the type [fin 2] has two values ([fO] and [fS
+   fO]), etc.  
+
+   Some definitions in this library are from equations example 
+   https://github.com/mattam82/Coq-Equations/blob/master/examples/Fin.v 
+
+*)
 
 (* ----------- imports --------------- *)
 Require Import Program.Basics Program.Combinators.
 From Equations Require Import Equations.
 Require Import Coq.Program.Equality. 
-
-(* these first few definitions are from equations example 
-   https://github.com/mattam82/Coq-Equations/blob/master/examples/Fin.v  *)
+Require Import Nat.
+Require Import Lia.
 
 Inductive fin : nat -> Set :=
   | fO : forall {n}, fin (S n)
@@ -21,140 +29,51 @@ Inductive fin : nat -> Set :=
 
 Derive Signature NoConfusionHom NoConfusion for fin.
 
-(** We can inject it into [nat]. *)
-Equations fog {n} (f : fin n) : nat :=
-fog (n:=?(S n)) (@fO n) := 0 ;
-fog (fS f) := S (fog f).
-
-(** The injection preserves the number: *)
-Lemma fog_inj {n} (f : fin n) : fog f < n.
-Proof with auto with arith. intros.
-  depind f; simp fog...
-Qed.
-
-(** Of course it has an inverse. *)
-
-(* coerce a natural number to the fin with the smallest possible 
-   range. *)
-Equations gof n : fin (S n) :=
-gof O := fO ;
-gof (S n) := fS (gof n).
-
-Lemma fog_gof n : fog (gof n) = n.
-Proof with auto with arith.
-  intros. funelim (gof n)... simp fog; congruence.
-Qed.
-
-Equations fin_inj_one {n} (f : fin n) : fin (S n) :=
-fin_inj_one fO := fO;
-fin_inj_one (fS f) := fS (fin_inj_one f).
-
-Inductive le : nat -> nat -> Type :=
-| le_O n : 0 <= n
-| le_S {n m} : n <= m -> S n <= S m
-where "n <= m" := (le n m).
-Derive Signature for le.
-
-Equations le_S_inv {n m} (p : S n <= S m) : n <= m :=
-le_S_inv (le_S p) := p.
-
-Equations fin_inj {n} {m} (f : fin n) (k : n <= m) : fin m :=
-fin_inj fO (le_S p) := fO;
-fin_inj (fS f) (le_S p) := fS (fin_inj f p).
-
-(** Let's do some arithmetic on [fin] *)
-
-Inductive finle : forall (n : nat) (x : fin n) (y : fin n), Prop :=
-| leqz : forall {n j}, finle (S n) fO j
-| leqs : forall {n i j}, finle n i j -> finle (S n) (fS i) (fS j).
-
-Scheme finle_ind_dep := Induction for finle Sort Prop.
-
-Instance finle_ind_pack n x y : DepElim.DependentEliminationPackage (finle n x y) :=
-  { elim_type := _ ; elim := finle_ind_dep }.
-
-Arguments finle {n}.
-
-(** Additional definitions and properties for fin *)
-
-(* equality is derivable *)
-
+(* decidable equality is derivable *)
 Derive EqDec for fin.
 
-(* 
-Equations fin_beq {n}  (f g : fin n) : bool :=
-  fin_beq fO fO := true;
-  fin_beq (n:=?(S n')) (fS f) (fS (n:=n') f')  := 
-    fin_beq f f';
-  fin_beq x y := false.
+(* ------- type coercions ------ *)
 
-Equations fin_eq_dec {n} (f g : fin n) : 
-   { f = g } + { f <> g } :=
-fin_eq_dec fO fO := left eq_refl;
-fin_eq_dec (n:=?(S n')) (fS f) (fS (n:=n') f') 
-  with fin_eq_dec f f' := 
-  { | left eq_refl => left eq_refl;
-    | right p => right _ };
-fin_eq_dec x y := right _.
-*)
-
-(* coerce m to a smaller range, as long as it is not 0. 
+(* Coerce m to a smaller range, as long as it is not 0. 
    does not change the value of m. *)
-(* used in "open" *)
+(* NB: used in "open" *)
 Equations decrease_fin (k : nat) (m : fin (S k)) : option (fin k) :=
   decrease_fin O _ := None ;
   decrease_fin (S _) fO := Some fO;
   decrease_fin (S m) (fS n) := option_map fS (decrease_fin m n).
 
-
-(* coerce m to a larger range. does not change the value of m. *)
-(* used in "close" operation. *)
+(* Coerce m to a larger range, without changing its value. *)
+(* NB: used in "close" operation. *)
 Equations increase_fin {n : nat} (m : fin n) : fin (S n) :=
   increase_fin (@fO n1) := fO;
   increase_fin (@fS n1 m) := fS (increase_fin m). 
 
-(* 
-pf : a + b = b + a
 
-match pf with 
- | eq_refl => ...
-end
+(* -------- isomorphism with {m : nat | m < n} ------- *)
 
-eta rules
+(** We can inject [fin n] into [nat]. Forget the rich type. *)
+Equations fog {n} (f : fin n) : nat :=
+  fog fO     := 0 ;
+  fog (fS f) := S (fog f).
 
-function:
-if a : A -> B then  a = \x. a x
+(** And come back again. Note: we produce a fin 
+    with the smallest possible range. *)
+Equations gof (n : nat) : fin (S n) :=
+  gof O := fO ;
+  gof (S n) := fS (gof n).
 
-[empty context]
-|- a : A -> B then  a ~>* \y. a'   [type soundness]
+(* -------- properties ------- *)
 
-    a = (\y.a')  ==?  \x. (\y.a') x  == \x. a'{x/y}
+Lemma fog_gof (n : nat) : fog (gof n) = n.
+Proof with auto with arith.
+  intros. funelim (gof n)... simp fog; congruence.
+Qed.
 
-product
-if a : A * B then a = (fst a, snd a)
+Lemma fog_inj {n} (f : fin n) : fog f < n.
+Proof with auto with arith. 
+  intros. depind f; simp fog...
+Qed.
 
-unit
-if a : unit  then a = ()
-
-equality type (axiom K)
-
-if a : A = B then a = refl
-
-
-
-*)
-
-(* coerce m to a much larger range. does not change the value of m. *)
-Equations weaken_fin {n : nat} (k:nat) (m : fin n) : fin (n + k) :=
-  weaken_fin k fO := fO ;
-  weaken_fin k (fS f) := fS (weaken_fin k f).
-(*
-Equations to_fin (n : nat) : fin (S n) :=
-  to_fin O     := fO ;
-  to_fin (S m) := fS (to_fin m).
-*)
-
-(* Theory *)
 
 (* increase_fin is injective *)
 Lemma increase_fin_inj : forall {n} (f f0 : fin n),
@@ -202,7 +121,8 @@ Qed.
 
 (* If we can decrease a fin, then increasing it gives us the same number. *)
 Lemma decrease_increase_fin :
-  forall {n1} (f0 : fin n1) (f : fin (S n1)),  decrease_fin n1 f = Some f0 -> increase_fin f0 = f.
+  forall {n1} (f0 : fin n1) (f : fin (S n1)),  
+    decrease_fin n1 f = Some f0 -> increase_fin f0 = f.
 Proof.
   intros.
   dependent induction f.
@@ -227,9 +147,9 @@ Proof.
   eapply IHf in E1; eauto. f_equal. auto.
 Qed.
 
-
-
-Lemma decrease_fin_increase_fin : forall n1 (f : fin n1), decrease_fin n1 (increase_fin f) = Some f.
+(* If we had increased first, we can decrease *)
+Lemma decrease_fin_increase_fin : 
+  forall n1 (f : fin n1), decrease_fin n1 (increase_fin f) = Some f.
 Proof. 
   intros.
   dependent induction f.
@@ -240,6 +160,8 @@ Proof.
   reflexivity.
 Qed.
 
+(* But since gof gives us the largest number in the range, we 
+   cannot decrease it. *)
 Lemma decrease_fin_gof : forall n, decrease_fin n (gof n) = None.
 Proof.
   induction n.
@@ -249,5 +171,10 @@ Proof.
   reflexivity.
 Qed.
 
-Hint Rewrite decrease_fin_increase_fin : decrease_fin.
-Hint Rewrite decrease_fin_gof : decrease_fin.
+Create HintDb fin.
+Hint Rewrite fog_gof : fin.
+Hint Rewrite decrease_fin_increase_fin : fin.
+Hint Rewrite decrease_fin_gof : fin.
+#[export] Hint Resolve decrease_to_fin : fin.
+#[export] Hint Resolve decrease_increase_fin : fin.
+#[export] Hint Resolve increase_not_n : fin.
