Stlc/Lemmas.v
@@ -22,7 +22,98 @@ Open Scope syntax_scope.
 
 Require Export Stlc.Definitions.
 
+(* Tactics for simplifying syntax definitions *)
 
+Ltac simp_stlc := repeat first [ 
+                       simp subst_exp_wrt_exp
+                     || simp open_exp_wrt_exp
+                     || simp close_exp_wrt_exp
+                     || simp weaken_exp
+                     || simpl size_exp
+                     || simpl fv_exp
+                     || simp increase_fin 
+                     || simp decrease_fin
+                     || simp fin
+                     ].
+
+Lemma fv_exp_var_b : forall n (m: fin n), fv (var_b m) = {}. 
+Proof. reflexivity. Qed.
+Lemma fv_exp_var_f : forall n (x:atom), fv (var_f (n:=n) x) = {{x}}.
+Proof. reflexivity. Qed.
+Lemma fv_exp_abs : forall n (e: exp (S n)), fv (abs e) = fv e.
+Proof. reflexivity. Qed.
+Lemma fv_exp_app : forall n (e1 : exp n) (e2: exp n), fv (app e1 e2) = fv e1 `union` fv e2.
+Proof. reflexivity. Qed.
+
+Hint Rewrite fv_exp_var_b fv_exp_var_f fv_exp_abs fv_exp_app : fv.
+
+(* Re-define behavior of size in terms of size_exp *)
+Lemma size_exp_var_b : forall n (m: fin n), size (var_b m) = 1. 
+Proof. reflexivity. Qed.
+Lemma size_exp_var_f : forall n (x:atom), size (var_f (n:=n) x) = 1.
+Proof. reflexivity. Qed.
+Lemma size_exp_abs : forall n (e: exp (S n)), size (abs e) = 1 + (size e).
+Proof. reflexivity. Qed.
+Lemma size_exp_app : forall n (e1 : exp n) (e2: exp n), size (app e1 e2) = 1 + size e1 + size e2.
+Proof. reflexivity. Qed.
+
+Hint Rewrite size_exp_var_b size_exp_var_f size_exp_abs size_exp_app : size.
+
+Lemma weaken_exp_var_b : forall n (m: fin n),   weaken  (var_b m) = var_b (increase_fin m).
+Proof. reflexivity. Qed.
+Lemma weaken_exp_var_f : forall n (x:atom), weaken (var_f (n:=n) x) = var_f x.
+Proof. reflexivity. Qed.
+Lemma weaken_exp_abs : forall n (e: exp (S n)), weaken (abs e) = abs (weaken e).
+Proof. reflexivity. Qed.
+Lemma weaken_exp_app : forall n (e1 : exp n) (e2: exp n), weaken (app e1 e2) = app (weaken e1) (weaken e2).
+Proof. reflexivity. Qed.
+
+Hint Rewrite weaken_exp_var_b weaken_exp_var_f weaken_exp_abs weaken_exp_app : weaken.
+
+Lemma close_exp_var_b : forall n x (m: fin n),   close x (var_b m) = var_b (increase_fin m).
+Proof. reflexivity. Qed.
+Lemma close_exp_var_f : forall n (x1 x2:atom), close x1 (var_f (n:=n) x2) = if (x1 == x2) then (var_b (gof n)) else (var_f x2).
+Proof. reflexivity. Qed.
+Lemma close_exp_abs : forall n (e: exp (S n)) x1, close x1 (abs e) = abs (close x1 e).
+Proof. reflexivity. Qed.
+Lemma close_exp_app : forall n (e1 : exp n) (e2: exp n) x1, close x1 (app e1 e2) = app (close x1 e1) (close x1 e2).
+Proof. reflexivity. Qed.
+
+Hint Rewrite close_exp_var_b close_exp_var_f close_exp_abs close_exp_app : close.
+
+Lemma open_exp_var_b : forall n (u:exp n) (m: fin (S n)), 
+    open u (var_b m) = 
+      match decrease_fin n m with
+      | Some f => var_b f
+      | None => u
+      end.
+Proof. reflexivity. Qed.
+Lemma open_exp_var_f : forall n (u:exp n) (x:atom), open u (var_f (n:= S n) x) = var_f x.
+Proof. reflexivity. Qed.
+
+Lemma open_exp_abs : forall n (u:exp n) (e: exp (S (S n))), 
+    open u (abs e) = abs (open (weaken u) e).
+Proof. reflexivity. Qed. 
+Lemma open_exp_app : forall n (u:exp n) (e1 : exp (S n)) (e2: exp (S n)), 
+    open u (app e1 e2) = app (open u e1) (open u e2).
+Proof. reflexivity. Qed.
+
+Hint Rewrite open_exp_var_b open_exp_var_f open_exp_abs open_exp_app : open.
+
+Lemma subst_exp_var_b : forall n (u:exp n) (y:atom) (m: fin n), 
+    subst u y (var_b m) = var_b m.
+Proof. reflexivity. Qed.
+Lemma subst_exp_var_f : forall n (u:exp n) (y:atom) (x:atom), 
+    subst u y (var_f (n:=n) x) = if x == y then u else var_f x.
+Proof. reflexivity. Qed.
+Lemma subst_exp_abs : forall n (u:exp n) (y:atom) (e: exp (S n)), 
+    subst u y (abs e) = abs (subst (weaken u) y e).
+Proof. reflexivity. Qed.
+Lemma subst_exp_app : forall n (u:exp n) (y:atom) (e1 : exp n) (e2: exp n), 
+    subst u y (app e1 e2) = app (subst u y e1) (subst u y e2).
+Proof. reflexivity. Qed.
+
+Hint Rewrite subst_exp_var_b subst_exp_var_f subst_exp_abs subst_exp_app : subst.
 
 
 (* *********************************************************************** *)
@@ -30,7 +121,9 @@ Require Export Stlc.Definitions.
 
 (** Additional hint declarations. *)
 
+(*
 #[global] Hint Resolve @plus_le_compat : lngen.
+*)
 
 (* Can't do this automatically b/c we need to have the 
    equality around. But then the option in the equality
@@ -57,13 +150,12 @@ Ltac default_case_split ::=
     | progress safe_f_equal
     ].
 
-Ltac default_auto ::= auto with arith lngen; tauto.
-Ltac default_autorewrite ::= simp_stlc.
-
 
 (* *********************************************************************** *)
 (** * Theorems about [weaken] *)
 
+Ltac default_auto ::= auto with arith lngen; tauto.
+Ltac default_autorewrite ::= simp_stlc.
 
 Lemma size_exp_weaken_exp :
 (forall n1 (e1 : exp n1),
@@ -169,8 +261,6 @@ dependent induction e1.
 all: simp_stlc.
 all: default_simp.
 destruct decrease_fin eqn:EQ; default_simp. 
-eauto using decrease_increase_fin.
-eauto using decrease_to_fin.
 Qed.
 
 #[global] Hint Resolve close_exp_wrt_exp_open_exp_wrt_exp : lngen.
@@ -198,7 +288,7 @@ Proof.
  intros k e2 e1 x1 FV1 FV2. 
  remember (var_f x1) as u.
  funelim (open_exp_wrt_exp u e2). 
- all: simp open_exp_wrt_exp.
+ all: simp_stlc. 
  all: intros h.
  all: match goal with [ |- _ = ?e ] => dependent elimination e end.
  all: simp open_exp_wrt_exp in h.
@@ -272,8 +362,6 @@ Qed.
 
 #[global] Hint Resolve fv_exp_open_exp_wrt_exp_lower : lngen.
 
-(* begin hide *)
-
 Lemma fv_exp_open_exp_wrt_exp_upper :
 (forall n1 (e1 : exp (S n1)) (e2 : exp n1),
   fv_exp (open_exp_wrt_exp e2 e1) [<=] fv_exp e2 `union` fv_exp e1).
@@ -308,8 +396,6 @@ fsetdec.
 Qed.
 
 #[global] Hint Resolve fv_exp_subst_exp_wrt_exp_lower : lngen.
-
-(* begin hide *)
 
 Lemma fv_exp_subst_exp_wrt_exp_notin :
 (forall n1 (e1 : exp n1) e2 x1 x2,
@@ -436,11 +522,13 @@ forall n1 (e2 : exp (S n1)) e1 x1 x2,
     subst_exp_wrt_exp e1 x1 (open_exp_wrt_exp (var_f x2) e2).
 Proof.
 intros; default_simp.
-Admitted.
+rewrite subst_exp_open_exp_wrt_exp.
+f_equal.
+simp subst.
+destruct (x2 == x1) eqn:E. subst. fsetdec. auto.
+Qed.
 
 #[global] Hint Resolve subst_exp_open_exp_wrt_exp_var : lngen.
-
-(* begin hide *)
 
 Lemma subst_exp_wrt_exp_spec :
 (forall n (e1 e2 : exp n) x1,
@@ -452,8 +540,6 @@ all: default_simp.
 Qed.
 
 #[global] Hint Resolve subst_exp_wrt_exp_spec : lngen.
-
-(* begin hide *)
 
 Lemma subst_exp_wrt_exp_subst_exp_wrt_exp :
 (forall n (e1 e2 e3 : exp n) x2 x1,
@@ -495,6 +581,7 @@ Qed.
 
 #[global] Hint Resolve subst_exp_wrt_exp_close_exp_wrt_exp_open_exp_wrt_exp : lngen.
 
+(*
 Lemma subst_exp_wrt_exp_abs :
 forall x2 (e2 : exp 1) (e1 : exp 0) x1,
   x2 `notin` fv_exp e1 `union` fv_exp e2 `union` singleton x1 ->
@@ -505,6 +592,7 @@ default_simp.
 Qed.
 
 #[global] Hint Resolve subst_exp_wrt_exp_abs : lngen.
+*)
 
 Lemma subst_exp_wrt_exp_intro :
 forall n1 (e1 : exp (S n1)) x1 e2,
@@ -525,43 +613,55 @@ Hint Rewrite subst_exp_wrt_exp_intro using solve [auto] : lngen.
 Ltac default_auto ::= auto; tauto.
 Ltac default_autorewrite ::= fail.
 
-#[global]
-Instance STE :  SyntaxTheory exp := {
+#[global] Instance STE :  SyntaxTheory exp := {
   size_weaken := size_exp_weaken_exp;
   fv_weaken := fv_exp_weaken_exp;
   size_min  := size_exp_min;
   size_close := size_exp_close_exp_wrt_exp;
   close_inj := close_exp_wrt_exp_inj;
-  close_weaken := close_exp_wrt_exp_weaken_exp
+  close_weaken := close_exp_wrt_exp_weaken_exp;
+  fv_close := fv_exp_close_exp_wrt_exp;
 }.
 
-(*
-  fv_close := fv_exp_close_exp_wrt_exp; *)
-(* TODO: fill in the rest *)
 
-#[global]
-Opaque STE.
+#[global] Opaque STE.
 
-#[global]
-Instance SSTE :  SubstTheory exp exp (@var_f) := {
+#[global] Instance SSTE : SubstTheory exp exp := {
   size_open := size_exp_open_exp_wrt_exp;
-  size_open_var := size_exp_open_exp_wrt_exp_var;
-  open_close := open_exp_wrt_exp_close_exp_wrt_exp;
-  open_inj := open_exp_wrt_exp_inj;
-  close_open := close_exp_wrt_exp_open_exp_wrt_exp;
   open_weaken := open_exp_wrt_exp_weaken_exp;
-(*
   fv_open_lower := fv_exp_open_exp_wrt_exp_lower;
   fv_open_upper := fv_exp_open_exp_wrt_exp_upper; 
   fv_subst_fresh := fv_exp_subst_exp_wrt_exp_fresh;
   fv_subst_lower := fv_exp_subst_exp_wrt_exp_lower;
   fv_subst_notin := fv_exp_subst_exp_wrt_exp_notin;
-  fv_subst_upper := fv_exp_subst_exp_wrt_exp_upper; *)
+  fv_subst_upper := fv_exp_subst_exp_wrt_exp_upper; 
 
-  subst_intro := subst_exp_wrt_exp_intro;
-  subst_open_var := subst_exp_open_exp_wrt_exp_var 
+  subst_close := subst_exp_close_exp_wrt_exp;
+  subst_fresh_eq := subst_exp_wrt_exp_fresh_eq;
+  subst_fresh_same := subst_exp_wrt_exp_fresh_same;
+  subst_weaken := subst_exp_wrt_exp_weaken_exp;
+  subst_spec := subst_exp_wrt_exp_spec;
 }.
-(* TODO: fill in the rest *)
 
-#[global]
-Opaque SSTE.
+
+#[global] Instance SVSTE :  SubstVarTheory exp exp (@var_f) := {
+  size_open_var := size_exp_open_exp_wrt_exp_var;
+  close_open := close_exp_wrt_exp_open_exp_wrt_exp;
+  open_close := open_exp_wrt_exp_close_exp_wrt_exp;
+  open_inj := open_exp_wrt_exp_inj;
+  subst_open_var := subst_exp_open_exp_wrt_exp_var;
+  subst_close_open := 
+    subst_exp_wrt_exp_close_exp_wrt_exp_open_exp_wrt_exp;
+  subst_intro := subst_exp_wrt_exp_intro;
+
+}.
+
+
+#[global] Opaque SVSTE.
+
+Instance SSSTE : SubstSubstTheory exp exp := {
+  subst_open := subst_exp_open_exp_wrt_exp;
+  subst_subst := subst_exp_wrt_exp_subst_exp_wrt_exp;
+}.
+
+#[global] Opaque SSSTE.
